P=O+tD\\
||P-P_0||=r\\
\\
(P-P_0)\cdot(P-P_0)=r^2\\
(O+tD-P_0)\cdot(O+tD-P_0)=r^2\\
\\
L=O-P_0\\
(L+tD)\cdot(L+tD)=r^2\\
\\
M=L+tD\\
M\cdot(L+tD)=r^2\\
M\cdot L+M\cdot tD=r^2\\
(L+tD)\cdot L+(L+tD)\cdot tD=r^2\\
L\cdot L+t(L \cdot D) +t(L \cdot D)+t^2(D\cdot D)=r^2\\
L\cdot L+2t(L \cdot D)+t^2(D\cdot D)=r^2\\
(O-P_0)\cdot (O-P_0)+2t((O-P_0) \cdot D)+t^2(D\cdot D)=r^2\\
(D\cdot D)t^2+2D\cdot (O-P_0)t+(O-P_0)\cdot (O-P_0)-r^2=0\\
\\
at^2+bt+c=0\\
\\
a = D\cdot D\\
b = 2D\cdot (O-P_0)\\
c = (O-P_0)\cdot (O-P_0)-r^2\\
\\
t=\frac{-b\pm\sqrt{b^2-4ac}}{2a}
